Fix DependentlyTypedMinimal

src/Parsers/DependentlyTypedMinimal.v
@@ -13,7 +13,8 @@ Section recursive_descent_parser.
   Context (CharType : Type)
           (String : string_like CharType)
           (G : grammar CharType).
-  Context {methods : @parser_computational_dataT _ String}.
+  Context {methods : @parser_computational_dataT _ String}
+          {strdata : @parser_computational_strdataT _ String G _ _}.
 
   Section minimal.
     Local Ltac t' :=
@@ -41,34 +42,34 @@ Section recursive_descent_parser.
     Section parts.
       Section common.
         Section types.
-          Context (str0 str : StringWithSplitState String split_stateT)
+          Context (str0 : String)
                   (valid : nonterminal_names_listT).
 
-          Definition T_nonterminal_name_success  (name : string) : Type
+          Definition T_nonterminal_name_success (name : string) (str : StringWithSplitState String (split_stateT (include_nonterminal_name _ name))) : Type
             := minimal_parse_of_name String G initial_nonterminal_names_data is_valid_nonterminal_name remove_nonterminal_name
                                      str0 valid str name.
-          Definition T_nonterminal_name_failure (name : string) : Type
-            := T_nonterminal_name_success name -> False.
+          Definition T_nonterminal_name_failure (name : string) str : Type
+            := T_nonterminal_name_success name str -> False.
 
-          Definition T_item_success (it : item CharType) : Type
+          Definition T_item_success (it : item CharType) (str : StringWithSplitState String (split_stateT it)) : Type
             := minimal_parse_of_item String G initial_nonterminal_names_data is_valid_nonterminal_name remove_nonterminal_name
                                      str0 valid str it.
-          Definition T_item_failure (it : item CharType) : Type
-            := T_item_success it -> False.
+          Definition T_item_failure (it : item CharType) str : Type
+            := T_item_success it str -> False.
 
-          Definition T_production_success (prod : production CharType) : Type
+          Definition T_production_success (prod : production CharType) (str : StringWithSplitState String (split_stateT prod)) : Type
             := minimal_parse_of_production String G initial_nonterminal_names_data is_valid_nonterminal_name remove_nonterminal_name
                                            str0 valid str prod.
 
-          Definition T_production_failure (prod : production CharType) : Type
-            := T_production_success prod -> False.
+          Definition T_production_failure (prod : production CharType) str : Type
+            := T_production_success prod str -> False.
 
-          Definition T_productions_success (prods : productions CharType) : Type
+          Definition T_productions_success (prods : productions CharType) (str : StringWithSplitState String (split_stateT prods)) : Type
             := minimal_parse_of String G initial_nonterminal_names_data is_valid_nonterminal_name remove_nonterminal_name
                                 str0 valid str prods.
 
-          Definition T_productions_failure (prods : productions CharType) : Type
-            := T_productions_success prods -> False.
+          Definition T_productions_failure (prods : productions CharType) str : Type
+            := T_productions_success prods str -> False.
         End types.
 
         Global Instance minimal_parser_dependent_types_data
@@ -84,33 +85,32 @@ Section recursive_descent_parser.
 
 
         Definition split_list_completeT
-                   (str0 : StringWithSplitState String split_stateT)
+                   (str0 : String)
                    valid1 valid2
-                   (str : StringWithSplitState String split_stateT) (pf : str ≤s str0)
-                   (split_list : list (StringWithSplitState String split_stateT * StringWithSplitState String split_stateT))
-                   (prod : production CharType)
-          := match prod return Type with
-               | nil => True
-               | it::its => ({ s1s2 : String * String
-                                      & (fst s1s2 ++ snd s1s2 =s str)
-                                        * (minimal_parse_of_item _ G initial_nonterminal_names_data is_valid_nonterminal_name remove_nonterminal_name str0 valid1 (fst s1s2) it)
-                                        * (minimal_parse_of_production _ G initial_nonterminal_names_data is_valid_nonterminal_name remove_nonterminal_name str0 valid2 (snd s1s2) its) }%type)
-                            -> ({ s1s2 : StringWithSplitState String split_stateT * StringWithSplitState String split_stateT
-                                         & (In s1s2 split_list)
-                                           * (minimal_parse_of_item _ G initial_nonterminal_names_data is_valid_nonterminal_name remove_nonterminal_name str0 valid1 (fst s1s2) it)
-                                           * (minimal_parse_of_production _ G initial_nonterminal_names_data is_valid_nonterminal_name remove_nonterminal_name str0 valid2 (snd s1s2) its) }%type)
-             end.
+                   (it : item CharType) (its : production CharType)
+                   (str : StringWithSplitState String (split_stateT (it::its : production CharType)))
+                   (pf : str ≤s str0)
+                   (split_list : list (StringWithSplitState String (split_stateT it) * StringWithSplitState String (split_stateT its)))
+          := ({ s1s2 : String * String
+                       & (fst s1s2 ++ snd s1s2 =s str)
+                         * (minimal_parse_of_item _ G initial_nonterminal_names_data is_valid_nonterminal_name remove_nonterminal_name str0 valid1 (fst s1s2) it)
+                         * (minimal_parse_of_production _ G initial_nonterminal_names_data is_valid_nonterminal_name remove_nonterminal_name str0 valid2 (snd s1s2) its) }%type)
+             -> ({ s1s2 : _
+                          & (In s1s2 split_list)
+                            * (minimal_parse_of_item _ G initial_nonterminal_names_data is_valid_nonterminal_name remove_nonterminal_name str0 valid1 (fst s1s2) it)
+                            * (minimal_parse_of_production _ G initial_nonterminal_names_data is_valid_nonterminal_name remove_nonterminal_name str0 valid2 (snd s1s2) its) }%type).
 
         Lemma H_prod_split'_helper
-              (str0 : StringWithSplitState String split_stateT)
+              (str0 : String)
               (valid : nonterminal_names_listT)
-              (it : item CharType) (its : list (item CharType))
-              (str strs : StringWithSplitState String split_stateT)
+              (it : item CharType) (its : production CharType)
+              (str : StringWithSplitState String (split_stateT it))
+              (strs : StringWithSplitState String (split_stateT its))
               (p_it : minimal_parse_of_item String G initial_nonterminal_names_data is_valid_nonterminal_name remove_nonterminal_name str0 valid str it)
               (p_its : minimal_parse_of_production String G initial_nonterminal_names_data is_valid_nonterminal_name remove_nonterminal_name str0 valid strs its)
               (ls : list
-                      (StringWithSplitState String split_stateT *
-                       StringWithSplitState String split_stateT))
+                      (StringWithSplitState String (split_stateT it) *
+                       StringWithSplitState String (split_stateT its)))
               (Hin : In (str, strs) ls)
               (H : fold_right
                      Datatypes.prod
@@ -119,9 +119,9 @@ Section recursive_descent_parser.
                         (fun s1s2 =>
                            let s1 := fst s1s2 in
                            let s2 := snd s1s2 in
-                           ((@T_item_failure str0 s1 valid it * @T_production_failure str0 s2 valid its)
-                            + (@T_item_success str0 s1 valid it * @T_production_failure str0 s2 valid its)
-                            + (@T_item_failure str0 s1 valid it * @T_production_success str0 s2 valid its))%type)
+                           ((@T_item_failure str0 valid it s1 * @T_production_failure str0 valid its s2)
+                            + (@T_item_success str0 valid it s1 * @T_production_failure str0 valid its s2)
+                            + (@T_item_failure str0 valid it s1 * @T_production_success str0 valid its s2))%type)
                         ls))
         : False.
         Proof.
@@ -134,11 +134,13 @@ Section recursive_descent_parser.
         Qed.
 
         Definition H_prod_split'
-                   (str0 str : StringWithSplitState String split_stateT)
+                   (str0 : String)
                    (valid : nonterminal_names_listT)
-                   pf it its
-                   (split_list_complete : @split_list_completeT str0 valid valid str pf (split_string_for_production str (it::its)) (it::its))
-        : @split_string_lift_T _ String _ str0 str valid it its (split_string_for_production str).
+                   it its
+                   (str : StringWithSplitState String (split_stateT (it::its : production CharType)))
+                   pf
+                   (split_list_complete : @split_list_completeT str0 valid valid it its str pf (split_string_for_production it its str))
+        : @split_string_lift_T _ String _ str0 valid it its str (split_string_for_production it its str).
         Proof.
           clear -split_list_complete.
           intros H pf' H'; hnf in H', split_list_complete.
@@ -160,22 +162,6 @@ Section recursive_descent_parser.
                  end.
           eapply H_prod_split'_helper; eassumption.
         Qed.
-
-        Definition H_prod_split''
-                   (str0 str : StringWithSplitState String split_stateT)
-                   (valid : nonterminal_names_listT)
-                   prod
-                   (split_list_complete : forall pf, @split_list_completeT str0 valid valid str pf (split_string_for_production str prod) prod)
-        : match prod return Type with
-            | nil => unit
-            | it::its => @split_string_lift_T _ String _ str0 str valid it its (split_string_for_production str)
-          end.
-        Proof.
-          unfold split_string_lift_T.
-          destruct prod.
-          { constructor. }
-          { intro pf. apply H_prod_split' with (pf := pf); try apply split_list_complete; assumption. }
-        Defined.
 
         Hint Constructors minimal_parse_of minimal_parse_of_name minimal_parse_of_production minimal_parse_of_item unit : minimal_instance_db.
 
@@ -215,22 +201,23 @@ Section recursive_descent_parser.
         Local Obligation Tactic := t.
 
         Global Program Instance minimal_parser_dependent_types_extra_data
-                (split_list_complete : forall str0 str valid prod pf, @split_list_completeT str0 valid valid str pf (split_string_for_production str prod) prod)
+                (split_list_complete : forall str0 valid it its str pf, @split_list_completeT str0 valid valid it its str pf (split_string_for_production it its str))
         : @parser_dependent_types_extra_dataT _ String G.
         Next Obligation.
-          hnf; apply H_prod_split''.
-          eauto.
+          eapply H_prod_split'; eauto.
+          Grab Existential Variables.
+          assumption.
         Defined.
       End common.
 
       Definition minimal_parse_nonterminal_name
                  (split_list_complete
-                  : forall str0 str valid prod pf,
-                      @split_list_completeT str0 valid valid str pf (split_string_for_production str prod) prod)
-      : forall (str : StringWithSplitState String split_stateT)
-               (nonterminal_name : string),
-          sum (T_nonterminal_name_success str str initial_nonterminal_names_data nonterminal_name)
-              (T_nonterminal_name_failure str str initial_nonterminal_names_data nonterminal_name)
+                  : forall str0 valid it its str pf,
+                      @split_list_completeT str0 valid valid it its str pf (split_string_for_production it its str))
+      : forall (nonterminal_name : string)
+               (str : StringWithSplitState String (split_stateT (include_nonterminal_name _ nonterminal_name))),
+          sum (T_nonterminal_name_success str initial_nonterminal_names_data nonterminal_name str)
+              (T_nonterminal_name_failure str initial_nonterminal_names_data nonterminal_name str)
         := @parse_nonterminal_name _ String G (minimal_parser_dependent_types_extra_data split_list_complete).
     End parts.
   End minimal.
